poSTVM/poSTVM_state_alt.thy
@@ -768,4 +768,5 @@ definition get_func :: "model_state \<Rightarrow> func_name \<Rightarrow> stacke
   (case st of (ST _ _ _ _ f_map) \<Rightarrow> the (fmlookup f_map name))"
 declare get_func_def [simp] 
 
+declare fmupd_reorder_neq [simp]
 end
