poST_Elevator.thy
@@ -1,0 +1,83 @@
+theory poST_Elevator
+  imports "~~/poST/poSTVM/poSTVM_alt_inductive"
+begin
+
+definition Elevator :: "model" where
+"Elevator = 
+  (None,[],
+  [(''Controller'',
+    [(program_var.InVar 
+      (fmap_of_list 
+        [(''onfloor0'',var_init_decl.Simple (basic_post_type.Bool False,None)),
+         (''onfloor1'',var_init_decl.Simple (basic_post_type.Bool False,None)),
+         (''onfloor2'',var_init_decl.Simple (basic_post_type.Bool False,None)),
+         (''call0'',var_init_decl.Simple (basic_post_type.Bool False,None)),
+         (''call1'',var_init_decl.Simple (basic_post_type.Bool False,None)),
+         (''call2'',var_init_decl.Simple (basic_post_type.Bool False,None)),
+         (''button0'',var_init_decl.Simple (basic_post_type.Bool False,None)),
+         (''button1'',var_init_decl.Simple (basic_post_type.Bool False,None)),
+         (''button2'',var_init_decl.Simple (basic_post_type.Bool False,None)),
+         (''door0closed'',var_init_decl.Simple (basic_post_type.Bool False,None)),
+         (''door1closed'',var_init_decl.Simple (basic_post_type.Bool False,None)),
+         (''door2closed'',var_init_decl.Simple (basic_post_type.Bool False,None))])),
+     (program_var.OutVar 
+      (fmap_of_list 
+        [(''up'',var_init_decl.Simple (basic_post_type.Bool False,None)),
+         (''down'',var_init_decl.Simple (basic_post_type.Bool False,None)),
+         (''open0'',var_init_decl.Simple (basic_post_type.Bool False,None)),
+         (''open1'',var_init_decl.Simple (basic_post_type.Bool False,None)),
+         (''open2'',var_init_decl.Simple (basic_post_type.Bool False,None)),
+         (''call0_LED'',var_init_decl.Simple (basic_post_type.Bool False,None)),
+         (''call1_LED'',var_init_decl.Simple (basic_post_type.Bool False,None)),
+         (''call2_LED'',var_init_decl.Simple (basic_post_type.Bool False,None)),
+         (''button0_LED'',var_init_decl.Simple (basic_post_type.Bool False,None)),
+         (''button1_LED'',var_init_decl.Simple (basic_post_type.Bool False,None)),
+         (''button2_LED'',var_init_decl.Simple (basic_post_type.Bool False,None)),
+         (''floor0_LED'',var_init_decl.Simple (basic_post_type.Bool False,None)),
+         (''floor1_LED'',var_init_decl.Simple (basic_post_type.Bool False,None)),
+         (''floor2_LED'',var_init_decl.Simple (basic_post_type.Bool False,None)),
+         (''cur'',var_init_decl.Simple (basic_post_type.Int 0,None))])),
+     (program_var.Var (False, 
+      (fmap_of_list 
+        [(''target'',var_init_decl.Simple (basic_post_type.Int 0,None))])))],
+    [(''Init'',
+      [],
+      [(''begin'',
+        False,
+        [(statement.ProcessSt (process_statement.Start (Some ''Call0Latch''))),
+         (statement.ProcessSt (process_statement.Start (Some ''Call1Latch''))),
+         (statement.ProcessSt (process_statement.Start (Some ''Call2Latch''))),
+         (statement.ProcessSt (process_statement.Start (Some ''Button0Latch''))),
+         (statement.ProcessSt (process_statement.Start (Some ''Button1Latch''))),
+         (statement.ProcessSt (process_statement.Start (Some ''Button2Latch''))),
+         (statement.ProcessSt (process_statement.Start (Some ''CheckCurFloor''))),
+         (statement.ProcessSt (process_statement.Start (Some ''UpControl''))),
+         (statement.ProcessSt (process_statement.Stop None))],
+        None)::state_decl])::process_decl,
+     (''Call0Latch'',
+      [(proc_var.Var (False,
+        (fmap_of_list
+          [(''prev_in'',var_init_decl.Simple (basic_post_type.Bool False,None)),
+           (''prev_out'',var_init_decl.Simple (basic_post_type.Bool False,None))])))],
+      [(''init'',
+        False,
+        [(statement.AssignSt (common_var.Symbolic ''prev_in'', expr.Unary (Some unary_op.Not) (expr.SymbolicVar ''call0''))),
+         (statement.AssignSt (common_var.Symbolic ''prev_out'', expr.Unary (Some unary_op.Not) (expr.SymbolicVar ''open0''))),
+         (statement.SetStateSt None)],
+        None),
+       (''check_ON_OFF'',
+        True,
+        [(statement.SelectSt (select_statement.IfSt
+                                [(expr.Binary (binary_op.And) (expr.SymbolicVar ''call0'') (expr.Unary (Some unary_op.Not) (expr.SymbolicVar ''prev_in'')),
+                                  [(statement.AssignSt (common_var.Symbolic ''call0_LED'', expr.Const (const.Bool True)))])]
+                                None)),
+         (statement.SelectSt (select_statement.IfSt
+                                [(expr.Binary (binary_op.And) (expr.SymbolicVar ''open0'') (expr.Unary (Some unary_op.Not) (expr.SymbolicVar ''prev_out'')),
+                                  [(statement.AssignSt (common_var.Symbolic ''call0_LED'', expr.Const (const.Bool False)))])]
+                                None)),
+         (statement.AssignSt (common_var.Symbolic ''prev_in'', expr.SymbolicVar ''call0'')),
+         (statement.AssignSt (common_var.Symbolic ''prev_out'', expr.SymbolicVar ''open0''))],
+        None)])])::program_decl],
+  [],[])"
+
+end
