poST_HandDryer.thy
@@ -1,0 +1,62 @@
+theory poST_HandDryer
+  imports "~~/poST/poSTVM/poSTVM_alt_inductive"
+begin
+
+
+definition HandDryer :: "model" where
+"HandDryer = 
+  (None,[],
+  [(''HandDryer'',
+    [(program_var.InVar (fmap_of_list [(''hands'',var_init_decl.Simple (basic_post_type.Bool False,None))])),
+     (program_var.OutVar (fmap_of_list [(''control'',var_init_decl.Simple (basic_post_type.Bool False,None))]))],
+    [(''HandDryer'',
+     [],
+     [(''Wait'',
+       False,
+       [(statement.SelectSt 
+          (select_statement.IfSt [(expr.SymbolicVar ''hands'',
+                                  [statement.AssignSt (common_var.Symbolic ''control'',expr.Const (const.Bool True)),
+                                   statement.SetStateSt None])] None))],
+       None),
+       (''Work'',
+        False,
+        [(statement.SelectSt 
+          (select_statement.IfSt [(expr.SymbolicVar ''hands'',
+                                  [statement.ResetSt])] None))],
+        Some (timeout_statement.Const 
+              (const.Time (time.Time 0 0 0 2 0))
+              [statement.AssignSt (common_var.Symbolic ''control'',expr.Const (const.Bool False)),
+               statement.SetStateSt None]))
+    :: state_decl]) 
+  :: process_decl]):: program_decl],
+  [],[]) "
+declare HandDryer_def [simp]
+
+definition stacked_HandDryer :: "stacked_model" where
+"stacked_HandDryer = stack_model HandDryer"
+declare stacked_HandDryer_def [simp]
+
+value "stacked_HandDryer"
+
+definition stacked_HandDaryer_model :: "model_state" where
+"stacked_HandDaryer_model = initialize_model_state stacked_HandDryer"
+declare stacked_HandDaryer_model_def [simp]
+
+value "stacked_HandDaryer_model"
+
+
+text "If the dryer is on, then it turns off after no hands are present for 1 second"
+text "If process time > 1s then control = false"
+definition rule1 :: "model_state \<Rightarrow> bool" where
+"rule1 st = 
+  ((time_more (get_time st ''HandDryer'') (time.Time 0 0 0 1 0)) \<longrightarrow> \<not>(basic_post_type_to_bool (get_symbvar_by_name st ''control''))) "
+declare rule1_def [simp]
+
+lemma "\<lbrakk>st = stacked_HandDaryer_model;
+        model = stacked_HandDryer\<rbrakk> \<Longrightarrow>\<forall>n::nat. (n\<Zspot>t:st\<turnstile>model\<mapsto>st1) \<longrightarrow> (rule1 st1)"
+  apply auto
+
+
+
+
+end
